Heap: Improved freshness interface.

theories/heap_lang/heap.v
@@ -2,7 +2,7 @@ From iris.prelude Require Import gmultiset.
 From iris.algebra Require Import auth gmap coPset csum agree.
 From iris.algebra Require Export gset frac.
 From iris.base_logic.lib Require Export invariants.
-From iris.base_logic.lib Require Import own auth fractional.
+From iris.base_logic.lib Require Import own fractional.
 From iris.base_logic Require Import big_op.
 From iris.heap_lang Require addenda.
 From iris.heap_lang Require Export on_val lifting.
@@ -14,106 +14,106 @@ Import addenda.lib_auth addenda.algebra_auth.
 
 Local Hint Resolve to_of_val.
 
+Definition heapN : namespace := nroot .@ "heap".
+
 (** The CMRAs we need. *)
 Local Notation heap := (gmap loc val).
-Definition heapN : namespace := nroot .@ "heap".
 Definition heapUR : ucmraT :=
   gmapUR loc (csumR (prodR fracR (agreeR valC)) unitR).
 Local Notation Hval q v := (Cinl (q%Qp, to_agree v)).
 Local Notation Lval := (Cinr ()).
-Local Notation locset := (gsetUR loc).
 
+Local Notation locset := (gset loc).
+Definition domUR : ucmraT := gmapUR loc (csumR (exclR unitR) unitR).
+Local Notation Fresh := (Cinl (Excl ())).
+Local Notation Live := (Cinr ()).
+
+Local Notation authG Σ R := (inG Σ (authR R)).
 Class heapG Σ := HeapG {
   heap_ownP_inG :> ownPG heap_lang Σ;
-  heap_liveG_inG :> inG Σ (authR locset);
-  heap_inG :> authG Σ heapUR;
+  heap_heapG_inG :> authG Σ heapUR;
+  heap_domG_inG :> authG Σ domUR;
   heap_name : gname * gname
 }.
 
 Class heapPreG Σ := HeapPreG {
   heap_preG_ownP_inG : ownPPreG heap_lang Σ;
-  heap_preG_liveG_inG : inG Σ (authR locset);
-  heap_preG_inG : authG Σ heapUR
+  heap_preG_heapG_inG : authG Σ heapUR;
+  heap_preG_domG_inG : authG Σ domUR
 }.
 (*
- * Lower priority than heapG's instances so the occurrence of
+ * Lower priority than [heapG]'s instances so the occurrence of
  * [heap_ctx] in the statement of [heap_adequacy] refers to the
  * "inner" [heapG] rather than the "outer" [heapPreG].
  *)
 Existing Instance heap_preG_ownP_inG | 30.
-Existing Instance heap_preG_liveG_inG | 30.
-Existing Instance heap_preG_inG | 30.
+Existing Instance heap_preG_heapG_inG | 30.
+Existing Instance heap_preG_domG_inG | 30.
 
-Definition heapΣ : gFunctors := #[
-  ownPΣ state; GFunctor (constRF (authR locset)); authΣ heapUR
-].
+Local Notation authΣ R := (GFunctor (constRF (authR R))).
+Definition heapΣ : gFunctors := #[ ownPΣ state; authΣ heapUR; authΣ domUR ].
 Instance subG_heapPreG {Σ} : subG heapΣ Σ → heapPreG Σ.
 Proof. intros [?[??]%subG_inv]%subG_inv. constructor; apply _. Qed.
 
-(** * Heap resources and invariant *)
+(** * Heap resources and the heap invariant *)
 Section definitions.
-  Context `{ownPG heap_lang Σ, inG Σ (authR locset), authG Σ heapUR}.
+  Context `{ownPG heap_lang Σ, authG Σ heapUR, authG Σ domUR}.
   Context (γ : gname * gname).
   Implicit Types l : loc.
   Implicit Types q : Qp.
   Implicit Types v : val.
   Implicit Types h : heap.
 
-  (** Live locations. *)
-  Definition liveloc'_def l : iProp Σ := own (γ.2) (◯ (to_gset {[ l ]})).
-  Definition liveloc'_aux : { x | x = @liveloc'_def }. by eexists. Qed.
-  Definition liveloc' := proj1_sig liveloc'_aux.
-  Definition liveloc'_eq : @liveloc' = @liveloc'_def := proj2_sig liveloc'_aux.
-
-  (** High locations. *)
-  Definition mapsto_def l q v : iProp Σ :=
-    (auth_own (γ.1) {[l := Hval q v]} ∗ liveloc' l)%I.
+  (** High vs low locations *)
+  Definition mapsto_def l q v : iProp Σ := own (γ.1) (◯ {[l := Hval q v]}).
   Definition mapsto_aux : { x | x = @mapsto_def }. by eexists. Qed.
   Definition mapsto := proj1_sig mapsto_aux.
   Definition mapsto_eq : @mapsto = @mapsto_def := proj2_sig mapsto_aux.
 
-  (** Low locations. *)
-  Definition lowloc'_def l : iProp Σ :=
-    (auth_own (γ.1) {[l := Lval]} ∗ liveloc' l)%I.
-  Definition lowloc'_aux : { x | x = @lowloc'_def }. by eexists. Qed.
-  Definition lowloc' := proj1_sig lowloc'_aux.
-  Definition lowloc'_eq : @lowloc' = @lowloc'_def := proj2_sig lowloc'_aux.
+  Definition lowloc_def l : iProp Σ := own (γ.1) (◯ ({[l := Lval]} : heapUR)).
+  Definition lowloc_aux : { x | x = @lowloc_def }. by eexists. Qed.
+  Definition lowloc' := proj1_sig lowloc_aux.
+  Definition lowloc_eq : @lowloc' = @lowloc_def := proj2_sig lowloc_aux.
 
-  (** Low values. *)
+  (** Low values *)
   Notation lowval' := (on_val lowloc').
 
+  (** Fresh vs live locations *)
+  Definition fresh_def l : iProp Σ := own (γ.2) (◯ {[l := Fresh]}).
+  Definition fresh_aux : { x | x = @fresh_def }. by eexists. Qed.
+  Definition fresh' := proj1_sig fresh_aux.
+  Definition fresh_eq : @fresh' = @fresh_def := proj2_sig fresh_aux.
+
+  Definition liveloc_def l : iProp Σ := own (γ.2) (◯ ({[l := Live]} : domUR)).
+  Definition liveloc_aux : { x | x = @liveloc_def }. by eexists. Qed.
+  Definition liveloc' := proj1_sig liveloc_aux.
+  Definition liveloc_eq : @liveloc' = @liveloc_def := proj2_sig liveloc_aux.
+
   (**
-    Invariant: The state is good and maps every high location to its
-    value and every low location to a low value. Locations are live
-    when they're in the heap's domain.
+	Invariant: The state is good and sends every high location to
+	its value and every low location to a low value. Orthogonally,
+	every location in the state's heap is either fresh or live.
   *)
+
   Definition to_high : heap → heapUR := fmap (λ v, Hval 1 v).
   Definition to_low : heap → heapUR  := fmap (λ _, Lval).
-  Definition to_heap (a : heap * heap) : heapUR :=
-    let: (h, h') := a in to_high h ⋅ to_low h'.
-  Definition hinv' (a : heap * heap) : iProp Σ := (
-    let: (h, h') := a in
-    ownP (good_state (h ∪ h'))
-    ∗ ([∗ map] v ∈ h', lowval' v)
-    ∗ own (γ.2) (● (dom (gset loc) (h ∪ h')))
+  Definition to_heap (h h' : heap) : heapUR := to_high h ⋅ to_low h'.
+
+  Definition to_fresh : locset → domUR := to_gmap Fresh.
+  Definition to_live : locset → domUR  := to_gmap Live.
+  Definition to_dom (L L' : locset) : domUR := to_fresh L ⋅ to_live L'.
+
+  Definition hinv' : iProp Σ := (
+    ∃ h h' L L', ⌜dom _ (h ∪ h') = L ∪ L'⌝ ∗
+    ownP (good_state (h ∪ h')) ∗
+    own (γ.1) (● to_heap h h') ∗ ([∗ map] v ∈ h', lowval' v) ∗
+    own (γ.2) (● to_dom L L')
   )%I.
-
-  Lemma hinv_alloc h :
-    ownP (good_state h) ∗ own (γ.2) (● dom (gset loc) h) ⊢ ▷ hinv' (h, ∅).
-  Proof.
-    rewrite /hinv' right_id big_sepM_empty left_id. exact: later_intro.
-  Qed.
-
-  Lemma to_heap_valid h : ✓ to_heap (h, ∅).
-  Proof. move=>l. rewrite lookup_op !lookup_fmap. by case (h !! l). Qed.
-
-  Definition heap_ctx' : iProp Σ := auth_ctx (γ.1) heapN to_heap hinv'.
+  Definition heap_ctx' : iProp Σ := inv heapN hinv'%I.
 
   Global Instance heap_ctx'_persistent : PersistentP heap_ctx'.
   Proof. apply _. Qed.
 End definitions.
-
-Notation liveloc := (liveloc' heap_name).
 
 Notation "l ↦{ q } v" := (mapsto heap_name l q v)
   (at level 20, q at level 50, format "l  ↦{ q }  v") : uPred_scope.
@@ -121,63 +121,46 @@ Notation "l ↦ v" := (mapsto heap_name l 1 v) (at level 20) : uPred_scope.
 Notation "l ↦{ q } -" := (∃ v, l ↦{q} v)%I
   (at level 20, q at level 50, format "l  ↦{ q }  -") : uPred_scope.
 Notation "l ↦ -" := (l ↦{1} -)%I (at level 20) : uPred_scope.
-
 Notation lowloc := (lowloc' heap_name).
 Notation lowval := (on_val lowloc).
-Notation heap_ctx := (heap_ctx' heap_name).
+Notation fresh := (fresh' heap_name).
+Notation liveloc := (liveloc' heap_name).
+Notation live L := ([∗ set] l ∈ L, liveloc l)%I (only parsing).
 Local Notation hinv := (hinv' heap_name).
+Notation heap_ctx := (heap_ctx' heap_name).
 
-(** Allocating the invariant. *)
-(** We cannot use [auth_alloc] as [hinv] depends on the ghost names. *)
-Lemma heap_ctx_alloc `{ownPG heap_lang Σ, inG Σ (authR locset), authG Σ heapUR} E h :
+(** We can establish the heap invariant. *)
+
+Lemma heap_ctx_alloc `{ownPG heap_lang Σ, authG Σ heapUR, authG Σ domUR} E h :
   ownP (good_state h) ={E}=∗ ∃ γ, heap_ctx' γ.
 Proof.
-  iIntros "Hσ". set h' := to_heap (h, ∅). set X := dom (gset loc) h.
-  iMod (own_alloc (Auth (Excl' h') h')) as (γheap) "Ha".
-  { split. done. exact: to_heap_valid. }
-  iMod (own_alloc (Auth (Excl' X) X)) as (γlive) "Hlive"; first done.
-  set γ := (γheap, γlive). set hinv_γ := @hinv' _ _ _ _ γ.
-  rewrite (auth_both_op h') (auth_both_op X).
-  iDestruct "Ha" as "[Ha _]". iDestruct "Hlive" as "[Hlive _]".
-  iDestruct (@hinv_alloc _ _ _ _ γ with "[$Hσ $Hlive]") as "Hh".
-  iMod (inv_alloc heapN _ (auth_inv γheap to_heap hinv_γ) with "[-]") as "#?".
-  { iNext. rewrite/auth_inv. iExists (h, ∅). by iFrame. }
-  iModIntro. iExists γ. by rewrite/heap_ctx'/auth_ctx.
+  iIntros "Hσ". set aH := to_heap h ∅. set aD := to_dom ∅ (dom _ h).
+  iMod (own_alloc (Auth (Excl' aH) aH)) as (γh) "Hh".
+  { split=>// l. rewrite lookup_op !lookup_fmap. by case (h !! l). }
+  iMod (own_alloc (Auth (Excl' aD) aD)) as (γd) "Hd".
+  { split=>// l. rewrite lookup_op !lookup_to_gmap.
+    rewrite option_guard_False // left_id.
+    case Hdom: (decide (l ∈ dom locset h)).
+    by rewrite option_guard_True. by rewrite option_guard_False. }
+  rewrite (auth_both_op aH). iDestruct "Hh" as "[Hh _]".
+  rewrite (auth_both_op aD). iDestruct "Hd" as "[Hd _]".
+  set γ := (γh, γd).
+  iMod (inv_alloc heapN _ (hinv' γ)%I with "[-]") as "?"; last by iExists γ.
+  iNext. iExists h, ∅, ∅, (dom _ h).
+  rewrite right_id big_sepM_empty union_empty_l_L.
+  by iFrame "Hσ Hh Hd".
 Qed.
 
-(** Observing good states. *)
+(** Under the heap invariant, we can observe the ambient state is good. *)
+
 Lemma heap_ctx_is_good `{heapG Σ} E :
  ↑heapN ⊆ E → heap_ctx ={E,∅}=∗ ∃ σ, ownP σ ∧ ⌜is_good σ⌝.
 Proof.
-  iIntros (?) "Hh". iMod (fupd_intro_mask' _ (↑heapN)) as "_"; first done.
-  iMod (auth_empty (heap_name.1)) as "Ha".
-  iMod (auth_open with "[$Hh $Ha]") as ([h h']) "(_&[>Hh _]&_)";
-    first done.
-  iExists _; iFrame. by rewrite subseteq_empty_difference_L.
+  iIntros (?) "Hctx". iMod (fupd_intro_mask' _ (↑heapN)) as "_"; first done.
+  iInv heapN as (h h' L L') "(_ & >Hσ & _ & _ & _)" "_".
+  rewrite subseteq_empty_difference_L //. iModIntro.
+  iExists (good_state (h ∪ h')). by iFrame "Hσ".
 Qed.
-
-(** Live locations *)
-Section live.
-  Context `{heapG Σ}.
-
-  Definition live : gset loc → iProp Σ := λ X, ([∗ set] l ∈ X, liveloc l)%I.
-
-  Global Instance liveloc_persistent l : PersistentP (liveloc l).
-  Proof. rewrite liveloc'_eq. apply _. Qed.
-  Global Instance liveloc_timeless l : TimelessP (liveloc l).
-  Proof. rewrite liveloc'_eq. apply _. Qed.
-
-  Global Instance live_persistent X : PersistentP (live X).
-  Proof. apply _. Qed.
-  Global Instance live_timeless X : TimelessP (live X).
-  Proof. apply _. Qed.
-
-  Lemma lowloc_live l : lowloc l ⊢ liveloc l.
-  Proof. by rewrite lowloc'_eq /lowloc'_def sep_elim_r. Qed.
-
-  Lemma mapsto_live l q v : l ↦{q} v ⊢ liveloc l.
-  Proof. by rewrite mapsto_eq /mapsto_def sep_elim_r. Qed.
-End live.
 
 (** * Low integrity predicates *)
 Class LowIntegrity Σ (A : Type) := Low {
@@ -200,17 +183,14 @@ Section low.
     (irreversible) ghost move [heap_mark_low].
   *)
   Global Instance lowloc_persistent l : PersistentP (lowloc l).
-  Proof. rewrite lowloc'_eq. apply _. Qed.
+  Proof. rewrite lowloc_eq. apply _. Qed.
   Global Instance lowloc_timeless l : TimelessP (lowloc l).
-  Proof. rewrite lowloc'_eq. apply _. Qed.
+  Proof. rewrite lowloc_eq. apply _. Qed.
   Global Instance loc_low : LowIntegrity Σ loc := Low lowloc _ _.
   Global Instance loc_low_timeless (l : loc) : TimelessP (low l).
   Proof. rewrite /low/=. apply _. Qed.
 
   Lemma low_loc l : low l ⊣⊢ lowloc l. Proof. by []. Qed.
-
-  Lemma low_live l : low l ⊢ liveloc l.
-  Proof. by rewrite low_loc lowloc_live. Qed.
 
   (** Low values lift low locations to values. *)
   Global Instance val_low : LowIntegrity Σ val := Low lowval _ _.
@@ -260,16 +240,8 @@ Ltac simpl_low :=
   end.
 Local Hint Extern 5 => simpl_low.
 
-(** * Bookkeeping lemmas *)
+(** * Bookkeeping *)
 Module internal.
-
-Notation Live h := (own (heap_name.2) (● dom (gset loc) h)) (only parsing).
-Notation HighLoc l q v := (auth_own (heap_name.1) {[l := Hval q v]})
-  (only parsing).
-Notation LowLoc l := (auth_own (heap_name.1) {[l := Lval ]}) (only parsing).
-Notation Phys h := (ownP (good_state h)) (only parsing).
-Notation Low h' := ([∗ map] v' ∈ h', low v')%I (only parsing).
-
 Section internal.
   Context `{heapG Σ}.
   Implicit Types l : loc.
@@ -277,18 +249,14 @@ Section internal.
   Implicit Types v : val.
   Implicit Types h : heap.
 
-  Remark to_heap_disjoint h h' : ✓ to_heap (h, h') → h ⊥ₘ h'.
-  Proof.
-    move=>Hv. rewrite map_disjoint_spec=>l ? ? EQ EQ'; move/(_ l): Hv.
-    by rewrite /to_heap lookup_op /to_high /to_low 2!lookup_fmap EQ EQ'.
-  Qed.
+  (** Map operations and [to_heap] *)
 
   Lemma lookup_to_high_None h l : h !! l = None → to_high h !! l = None.
   Proof. by rewrite /to_high lookup_fmap=> ->. Qed.
   Lemma lookup_to_low_None h l : h !! l = None → to_low h !! l = None.
   Proof. by rewrite /to_low lookup_fmap=> ->. Qed.
   Lemma lookup_to_heap_None h h' l :
-    (h ∪ h') !! l = None → to_heap (h, h') !! l = None.
+    (h ∪ h') !! l = None → to_heap h h' !! l = None.
   Proof.
     move=> /lookup_union_None [??].
     by rewrite lookup_op lookup_to_high_None ?lookup_to_low_None.
@@ -300,18 +268,164 @@ Section internal.
   Lemma lookup_to_low_Some h l v : h !! l = Some v → to_low h !! l = Some Lval.
   Proof. by rewrite /to_low lookup_fmap=>->. Qed.
   Lemma lookup_to_heap_Some h h' l v :
-    h !! l = Some v → h' !! l = None → to_heap (h, h') !! l = Some (Hval 1 v).
+    h !! l = Some v → h' !! l = None → to_heap h h' !! l = Some (Hval 1 v).
   Proof.
     rewrite /to_heap lookup_op.
     by move=>/lookup_to_high_Some->/lookup_to_low_None->.
   Qed.
 
+  Lemma to_heap_high_insert h h' l v :
+    h' !! l = None →
+    to_heap (<[l:=v]> h) h' = <[l:=Hval 1 v]> (to_heap h h').
+  Proof.
+    move=>?. rewrite /to_heap /to_high fmap_insert. apply/map_eq => l'.
+    case: (decide (l = l'))=> [<-|?].
+    - rewrite insert_op_l //. by rewrite lookup_to_low_None.
+    - by rewrite lookup_op lookup_insert_ne // lookup_insert_ne // -lookup_op.
+  Qed.
+  Lemma to_heap_low_insert h h' l v :
+    h !! l = None → to_heap h (<[l:=v]> h') = <[l:=Lval]>(to_heap h h').
+  Proof.
+    move=>?. rewrite /to_heap /to_low fmap_insert. apply/map_eq=> l'.
+    case: (decide (l = l'))=> [<-|?].
+    - rewrite insert_op_r //. by rewrite lookup_to_high_None.
+    - by rewrite lookup_op lookup_insert_ne // lookup_insert_ne // -lookup_op.
+  Qed.
+  Lemma to_heap_low_insert_override h h' l v1 v2 :
+    h' !! l = Some v1 → to_heap h h' = to_heap h (<[l:=v2]> h').
+  Proof.
+    move=>Hlow. apply/map_eq=> l'. rewrite 2!lookup_op. f_equiv.
+    rewrite /to_low 2!lookup_fmap. case: (decide (l = l')) =>[<-|?].
+    - by rewrite Hlow lookup_insert.
+    - by rewrite lookup_insert_ne.
+  Qed.
+
+  Lemma to_heap_delete h h' l :
+    h' !! l = None →
+    delete l (to_heap h h') = to_heap (delete l h) h'.
+  Proof.
+    move=>Hdom. rewrite /to_heap /to_high fmap_delete.
+    apply/map_eq=> l'. rewrite lookup_op. case: (decide (l = l'))=> [<-|?].
+    - by rewrite !lookup_delete lookup_to_low_None.
+    - by rewrite lookup_delete_ne // lookup_delete_ne // -lookup_op.
+  Qed.
+
+  (** Set operations and [to_dom] *)
+
+  Local Ltac crack l L :=
+    case: (decide (l ∈ L))=>?;
+    [rewrite option_guard_True //|rewrite option_guard_False //].
+
+  Lemma lookup_to_fresh_None L l : l ∉ L → to_fresh L !! l = None.
+  Proof. move=>?. by rewrite lookup_to_gmap option_guard_False. Qed.
+  Lemma lookup_to_live_None L' l : l ∉ L' → to_live L' !! l = None.
+  Proof. move=>?. by rewrite lookup_to_gmap option_guard_False. Qed.
+  Lemma lookup_to_dom_None L L' l : l ∉ L ∪ L' → to_dom L L' !! l = None.
+  Proof.
+    move/not_elem_of_union=>[??].
+    by rewrite lookup_op lookup_to_fresh_None // lookup_to_live_None.
+  Qed.
+
+  Lemma to_dom_fresh_insert L L' l :
+    l ∉ L' → to_dom ({[l]} ∪ L) L' = <[l:=Fresh]> (to_dom L L').
+  Proof.
+    move=>?. rewrite/to_dom/to_fresh to_gmap_union_singleton.
+    by rewrite insert_op_l // lookup_to_live_None.
+  Qed.
+
+  Lemma to_dom_delete L L' l :
+    l ∉ L' → delete l (to_dom L L') = to_dom (L ∖ {[l]}) L'.
+  Proof.
+    move=>?. apply/map_eq=> x. rewrite lookup_op 2!lookup_to_gmap.
+    case: (decide (l = x))=>[<-|?].
+    - by rewrite lookup_delete // !option_guard_False //
+        elem_of_difference elem_of_singleton =>-[].
+    - rewrite lookup_delete_ne //.
+      rewrite lookup_op 2!lookup_to_gmap. f_equal. crack x L.
+      + by rewrite option_guard_True // elem_of_difference
+          elem_of_singleton.
+      + rewrite option_guard_False // elem_of_difference. by case; auto.
+  Qed.
+
+  Lemma to_dom_live_insert L L' l :
+    to_dom (L ∖ {[l]}) ({[l]} ∪ L') = <[l:=Live]> (to_dom (L ∖ {[l]}) L').
+  Proof.
+    apply/map_eq=>x. rewrite lookup_op !lookup_to_gmap.
+    case: (decide (l = x))=>[<-|?].
+    - rewrite lookup_insert option_guard_False.
+      + rewrite option_guard_True // elem_of_union elem_of_singleton.
+        by left.
+      + rewrite not_elem_of_difference elem_of_singleton. by right.
+    - rewrite lookup_insert_ne // lookup_op 2!lookup_to_gmap.
+      f_equal. crack x L'.
+      + by rewrite option_guard_True.
+      + rewrite elem_of_union. by right.
+      + by rewrite option_guard_False.
+      + by rewrite not_elem_of_union not_elem_of_singleton.
+  Qed.
+
+  Lemma dom_mark_live h h' L L' l :
+    l ∈ L → dom locset (h ∪ h') = L ∪ L' →
+    dom locset (h ∪ h') = L ∖ {[l]} ∪ ({[l]} ∪ L').
+  Proof.
+    move=>?->. set L'' := L ∖ {[l]}. unfold_leibniz=>x. rewrite elem_of_union.
+    by case: (decide (l = x))=>[<-|?]; set_solver.
+  Qed.
+
+  Lemma dom_alloc_fresh h h' L L' l v :
+    (h ∪ h') !! l = None → dom locset (h ∪ h') = L ∪ L' →
+    dom locset (<[l:=v]> h ∪ h') = {[l]} ∪ L∪ L'.
+  Proof.
+    move=>? HD. unfold_leibniz=>x. rewrite -assoc -HD. fold_leibniz.
+    rewrite -insert_union_l elem_of_union elem_of_singleton !elem_of_dom.
+    split=>[-[] u|[?|-[] u]]; case: (decide (l = x))=>[<-|?].
+    - move=>_. by left.
+    - rewrite lookup_insert_ne // => ?. by right; exists u.
+    - subst. exists v. by rewrite lookup_insert.
+    - done.
+    - move=>_. exists v. by rewrite lookup_insert.
+    - move=>?. exists u. by rewrite lookup_insert_ne.
+  Qed.
+
+  Lemma dom_store_high h h' L L' l v1 v2 :
+    h !! l = Some v1 → h' !! l = None → dom locset (h ∪ h') = L ∪ L' →
+    dom locset (<[l:=v2]> h ∪ h') = L ∪ L'.
+  Proof.
+    move=>?? <-. unfold_leibniz=>x. fold_leibniz.
+    rewrite !elem_of_dom. split=>-[] u; case: (decide (l = x))=>[<-|?].
+    - move=>_. exists v1. exact: lookup_union_Some_l.
+    - rewrite -insert_union_l lookup_insert_ne // =>?. by exists u.
+    - move=>_. exists v2. by rewrite -insert_union_l lookup_insert.
+    - move=>?. exists u. by rewrite -insert_union_l lookup_insert_ne.
+  Qed.
+
+  Lemma dom_low_insert_override h h' L L' l v1 v2 :
+    h !! l = None → h' !! l = Some v1 → dom locset (h ∪ h') = L ∪ L' →
+    dom locset (h ∪ <[l:=v2]> h') = L ∪ L'.
+  Proof.
+    move=>?? <-. unfold_leibniz=>x. fold_leibniz.
+    rewrite !elem_of_dom -insert_union_r //.
+    split=>-[] u; case: (decide (l = x))=>[<-|?].
+    - move=>_. exists v1. exact: lookup_union_Some_r'.
+    - rewrite lookup_insert_ne // => ?. by exists u.
+    - move=>_. exists v2. by rewrite lookup_insert.
+    - move=>?. exists u. by rewrite lookup_insert_ne.
+  Qed.
+
+  (** Validity *)
+
+  Remark to_heap_disjoint h h' : ✓ to_heap h h' → h ⊥ₘ h'.
+  Proof.
+    move=>Hv. rewrite map_disjoint_spec=>l ? ? EQ EQ'; move/(_ l): Hv.
+    by rewrite /to_heap lookup_op /to_high /to_low 2!lookup_fmap EQ EQ'.
+  Qed.
+
   Lemma to_heap_high_included h h' l q v :
-    ✓ to_heap (h, h') → {[l := Hval q v]} ≼ to_heap (h, h') →
+    ✓ to_heap h h' → {[l := Hval q v]} ≼ to_heap h h' →
     h !! l = Some v ∧ h' !! l = None.
   Proof.
     rewrite singleton_included => /(_ l) Hv [] u []; move: Hv.
-    rewrite !lookup_op /to_high /to_low !lookup_fmap.
+    rewrite !lookup_op !lookup_fmap.
     case EQ: (h !! l)=>[vh|]; case EQ': (h' !! l)=>[vl|] /=.
     - by rewrite -Some_op Some_valid.
     - rewrite right_id.
@@ -336,7 +450,7 @@ Section internal.
   Qed.
 
   Lemma to_heap_low_included h h' l :
-    ✓ to_heap (h, h') → {[l := Lval]} ≼ to_heap (h, h') →
+    ✓ to_heap h h' → {[l := Lval]} ≼ to_heap h h' →
     h !! l = None ∧ is_Some(h' !! l).
   Proof.
     rewrite singleton_included => /(_ l) Hv [] u []; move: Hv.
@@ -352,48 +466,24 @@ Section internal.
     - rewrite right_id. by move=> _ /option_equivE.
   Qed.
 
-  Lemma to_heap_high_insert h h' l v :
-    h' !! l = None →
-    to_heap (<[l:=v]> h, h') = <[l:=Hval 1 v]>(to_heap (h, h')).
+  Lemma to_dom_fresh_included L L' l :
+    ✓ to_dom L L' → {[l := Fresh]} ≼ to_dom L L' → l ∈ L ∧ l ∉ L'.
   Proof.
-    move=>?. rewrite /to_heap /to_high fmap_insert. apply/map_eq => l'.
-    case: (decide (l = l'))=> [<-|?].
-    - rewrite insert_op_l //. by rewrite lookup_to_low_None.
-    - by rewrite lookup_op lookup_insert_ne // lookup_insert_ne // -lookup_op.
+    rewrite singleton_included => /(_ l) Hv [] u []; move: Hv.
+    rewrite !lookup_op !lookup_to_gmap.
+    crack l L; crack l L'; rewrite left_id.
+    - case=>EQ. apply Some_equiv_inj in EQ. rewrite -EQ.
+      case/Some_included; first by move/csum_equivE.
+      by case/csum_included => // -[] [] ? [] ? [] ? [] ?.
+    - by move=>_ /option_equivE.
   Qed.
 
-  Lemma to_heap_low_insert h h' l v :
-    h !! l = None → to_heap (h, <[l:=v]> h') = <[l:=Lval]>(to_heap (h, h')).
-  Proof.
-    move=>?. rewrite /to_heap /to_low fmap_insert. apply/map_eq=> l'.
-    case: (decide (l = l'))=> [<-|?].
-    - rewrite insert_op_r //. by rewrite lookup_to_high_None.
-    - by rewrite lookup_op lookup_insert_ne // lookup_insert_ne // -lookup_op.
-  Qed.
-
-  Lemma to_heap_low_insert_override h h' l v1 v2 :
-    h' !! l = Some v1 → to_heap (h, h') = to_heap (h, <[l:=v2]> h').
-  Proof.
-    move=>Hlow. apply/map_eq=> l'. rewrite 2!lookup_op. f_equiv.
-    rewrite /to_low 2!lookup_fmap. case: (decide (l = l')) =>[<-|?].
-    - by rewrite Hlow lookup_insert.
-    - by rewrite lookup_insert_ne.
-  Qed.
-
-  Lemma to_heap_delete h h' l :
-    h' !! l = None →
-    delete l (to_heap (h, h')) = to_heap (delete l h, h').
-  Proof.
-    move=>Hdom. rewrite /to_heap /to_high fmap_delete.
-    apply/map_eq=> l'. rewrite lookup_op. case: (decide (l = l'))=> [<-|?].
-    - by rewrite !lookup_delete lookup_to_low_None.
-    - by rewrite lookup_delete_ne // lookup_delete_ne // -lookup_op.
-  Qed.
+  (** Updates *)
 
   Lemma to_heap_mark_low h h' l v :
-    ✓ to_heap (h, h') → {[l := Hval 1 v]} ≼ to_heap (h, h') →
-    (to_heap (h, h'), {[l := Hval 1 v]}) ~l~>
-    (to_heap (delete l h, <[l:=v]> h'), {[l := Lval]}).
+    ✓ to_heap h h' → {[l := Hval 1 v]} ≼ to_heap h h' →
+    (to_heap h h', {[l := Hval 1 v]}) ~l~>
+    (to_heap (delete l h) (<[l:=v]> h'), {[l := Lval]}).
   Proof.
     move=>Hv /to_heap_high_included -/(_ Hv)[_ ?].
     etransitivity; first by apply delete_singleton_local_update, _.
@@ -402,130 +492,46 @@ Section internal.
     apply lookup_to_heap_None, lookup_union_None. by rewrite lookup_delete.
   Qed.
 
-  Lemma high_eq l q v : l ↦{q} v ⊣⊢ HighLoc l q v ∗ liveloc l.
-  Proof. by rewrite mapsto_eq. Qed.
-
-  Lemma high_HighLoc l q v : l ↦{q} v ⊢ HighLoc l q v.
-  Proof. by rewrite high_eq sep_elim_l. Qed.
-
-  Lemma low_eq l : low l ⊣⊢ LowLoc l ∗ liveloc l.
-  Proof. by rewrite low_loc lowloc'_eq. Qed.
-
-  Lemma hinv_mark_low h h' l v :
-    ✓ to_heap (h, h') → {[l := Hval 1 v]} ≼ to_heap (h, h') →
-    ▷ low v -∗ ▷ Phys (h ∪ h') -∗ ▷ Low h' -∗ ▷ Live (h ∪ h') -∗
-    ▷ hinv (delete l h, <[l:=v]> h').
+  Lemma to_dom_mark_live L L' l :
+    ✓ to_dom L L' → {[l := Fresh]} ≼ to_dom L L' →
+    (to_dom L L', {[l := Fresh]}) ~l~>
+    (to_dom (L ∖ {[l]}) ({[l]} ∪ L'), {[l := Live]}).
   Proof.
-    move=>Hv /to_heap_high_included -/(_ Hv)[??]. rewrite/hinv.
-    iIntros "Hv Hσ Hlow Hlive". rewrite -delete_insert_union //.
-    iFrame. rewrite 2!big_sepM_later big_sepM_insert //. by iFrame.
+    move=>Hv /to_dom_fresh_included -/(_ Hv)[_ ?].
+    etransitivity; first by apply delete_singleton_local_update, _.
+    rewrite to_dom_delete // to_dom_live_insert.
+    apply alloc_singleton_local_update; last done.
+    rewrite lookup_op !lookup_to_gmap !option_guard_False //.
+    rewrite not_elem_of_difference elem_of_singleton. by right.
   Qed.
-
-  (* PDS: Hoist. *)
-  Lemma to_gset_singleton l : to_gset {[l]} = {[l]}.
-  Proof.
-    apply mapset_eq=> x. rewrite elem_of_to_gset; last exact: singleton_finite.
-    by rewrite 2!elem_of_singleton.
-  Qed.
-
-  Lemma live_obs h l X :
-    h !! l = None →
-    Live h -∗ live X -∗ ⌜l ∉ X⌝.
-  Proof.
-    rewrite/live liveloc'_eq /liveloc'_def=>Hdom.
-    induction X as [|x X Hx IH] using collection_ind_L.
-    { iIntros "Hh _". iPureIntro. exact: not_elem_of_empty. }
-    iIntros "Hh HX".
-    rewrite big_sepS_union; last by move=>?/elem_of_singleton->.
-    rewrite big_sepS_singleton. iDestruct "HX" as "(Hx & HX)".
-    iDestruct (IH with "Hh HX") as "%". rewrite not_elem_of_union.
-    case: (decide (l = x))=>?; last first.
-    { iFrame. iPureIntro. by rewrite not_elem_of_singleton. }
-    subst. iExFalso. iDestruct (own_valid_2 with "Hh Hx") as "Hv".
-    iDestruct "Hv" as %[Hinc%gset_included _]%auth_valid_discrete_2.
-    iPureIntro. move: Hinc=>/(_ x).
-    rewrite (to_gset_singleton x) elem_of_singleton=>
-      /(_ (eq_refl _))/elem_of_dom.
-    by rewrite Hdom=>-[].
-  Qed.
-
-  Lemma live_alloc h l v :
-    Live h ==∗ Live (<[l:=v]> h) ∗ liveloc l.
-  Proof.
-    rewrite/live liveloc'_eq /liveloc'_def.
-    rewrite -(sep_elim_r (own (heap_name.2) (◯ dom (gset loc) h))
-      (own _ (◯ to_gset {[l]}))) -2!own_op -auth_frag_op.
-    apply own_update, auth_update_alloc.
-    rewrite dom_insert comm gset_op_union (to_gset_singleton l).
-    apply gset_local_update, union_subseteq_l.
-  Qed.
-
-  Lemma hinv_high h h' l v :
-    Phys (<[l:=v]> (h ∪ h')) -∗ Low h' -∗ Live (<[l:=v]> (h ∪ h')) -∗
-    hinv (<[l:=v]> h, h').
-  Proof. rewrite/hinv insert_union_l. by iIntros; iFrame. Qed.
-
-  Lemma hinv_intro h h' :
-    Phys (h ∪ h') -∗ Low h' -∗ Live (h ∪ h') -∗ hinv (h, h').
-  Proof. rewrite/hinv. by iIntros; iFrame. Qed.
 
   Lemma to_heap_alloc_high h h' l v :
     (h ∪ h') !! l = None →
-    (to_heap (h, h'), ∅) ~l~> (to_heap (<[l:=v]> h, h'), {[l := Hval 1 v]}).
+    (to_heap h h', ∅) ~l~> (to_heap (<[l:=v]> h) h', {[l := Hval 1 v]}).
   Proof.
     move=>Hdom.
     rewrite to_heap_high_insert; last by move: Hdom=>/lookup_union_None[].
-    apply alloc_singleton_local_update; last done.
-    by apply lookup_to_heap_None.
+    apply alloc_singleton_local_update. by apply lookup_to_heap_None. done.
   Qed.
 
-  Lemma live_store_high h h' l v' v :
-    h !! l = Some v' → h' !! l = None →
-    Live (h ∪ h') ⊣⊢ Live (<[l:=v]> (h ∪ h')).
+  Lemma to_dom_alloc_fresh L L' l :
+    l ∉ L ∪ L' →
+    (to_dom L L', ∅) ~l~> (to_dom ({[l]} ∪ L) L', {[l := Fresh]}).
   Proof.
-    move=>??. do 4!f_equiv. apply mapset_eq=>x. rewrite 2!elem_of_dom.
-    case: (decide (x = l))=>?.
-    - subst. simplify_map_eq. by rewrite 2!is_Some_alt.
-    - by rewrite lookup_insert_ne.
+    move=>Hdom. rewrite to_dom_fresh_insert;
+      last by move: Hdom=>/not_elem_of_union [].
+    apply alloc_singleton_local_update; last done.
+    by apply lookup_to_dom_None.
   Qed.
 
   Lemma to_heap_store_high h h' l v1 v2 :
-    ✓ to_heap (h, h') → h !! l = Some v1 → h' !! l = None →
-    (to_heap (h, h'), {[l := Hval 1 v1]}) ~l~>
-    (to_heap (<[l:=v2]> h, h'), {[l := Hval 1 v2]}).
+    ✓ to_heap h h' → h !! l = Some v1 → h' !! l = None →
+    (to_heap h h', {[l := Hval 1 v1]}) ~l~>
+    (to_heap (<[l:=v2]> h) h', {[l := Hval 1 v2]}).
   Proof.
     move=>???. rewrite to_heap_high_insert //.
     eapply singleton_local_update; first exact: lookup_to_heap_Some.
     exact: exclusive_local_update.
-  Qed.
-
-  Lemma live_store_low h h' l v1 v2 :
-    h !! l = None → h' !! l = Some v1 →
-    Live (h ∪ h') ⊣⊢ Live (h ∪ <[l:=v2]> h').
-  Proof.
-    move=>Hhigh Hlow.
-    do 4!f_equiv. apply mapset_eq=>x. rewrite 2!elem_of_dom.
-    case: (decide (x = l))=>?.
-    - subst. rewrite (lookup_union_Some_r' _ _ _ v1) //.
-      rewrite (lookup_union_Some_r' _ _ _ v2) //.
-      by rewrite 2!is_Some_alt.  by rewrite lookup_insert.
-    - case Hleft: (h !! x) => [v|]; first by simplify_map_eq.
-      case Hright: (h' !! x) => [v'|].
-      + do 2!rewrite (lookup_union_Some_r' _ _ _ v') //.
-        by rewrite lookup_insert_ne.
-      + have->: (h ∪ h') !! x = None by apply lookup_union_None.
-        have->: (h ∪ <[l:=v2]> h') !! x = None; last done.
-        apply lookup_union_None. by rewrite lookup_insert_ne.
-  Qed.
-
-  Lemma hinv_store_low h h' l v1 v2 :
-    h !! l = None → h' !! l = Some v1 →
-    low v2 -∗ Phys (<[l:=v2]> (h ∪ h')) -∗ Low h' -∗ Live (h ∪ <[l:=v2]> h') -∗
-    hinv (h, <[l:=v2]> h').
-  Proof.
-    move=>??.
-    rewrite /hinv insert_union_r // big_sepM_insert_override_2 //.
-    iIntros "? ? Hlow ?". iFrame. iApply "Hlow". eauto.
   Qed.
 End internal.
 End internal.
@@ -540,28 +546,13 @@ Section heap.
   Import internal.
 
   (** ** Structure *)
-  (**
-	High locations and the heap context enjoy their usual
-	properties. Low locations are timeless, persistent, and
-	disjoint from high locations. High locations containing low
-	values can be marked low.
-  *)
-  Lemma high_not_low l q v : l ↦{q} v ∗ low l ⊢ False.
-  Proof.
-    rewrite high_HighLoc low_eq (sep_elim_l _ (liveloc _)).
-    rewrite -auth_own_op auth_own_valid discrete_valid.
-    by rewrite op_singleton singleton_valid.
-  Qed.
+  (** High locations enjoy their usual properties. *)
 
   Global Instance mapsto_timeless l q v : TimelessP (l ↦{q} v).
   Proof. rewrite mapsto_eq. apply _. Qed.
   Global Instance mapsto_fractional l v : Fractional (λ q, l ↦{q} v)%I.
   Proof.
-    enough (F : Fractional (λ q, HighLoc l q v)).
-    { intros p q. rewrite 3!high_eq. iSplit.
-      - iIntros "(Hpq & #HL)". iFrame "HL HL". by rewrite -F.
-      - iIntros "([Hp _] & Hq & HL)". rewrite (F p q). by iFrame "Hp Hq HL". }
-    intros p q. rewrite -auth_own_op.
+    intros p q. rewrite mapsto_eq -own_op -auth_frag_op.
     by rewrite op_singleton Cinl_op pair_op agree_idemp.
   Qed.
   Global Instance mapsto_as_fractional l q v :
@@ -570,9 +561,10 @@ Section heap.
 
   Lemma mapsto_agree l q1 q2 v1 v2 : l ↦{q1} v1 ∗ l ↦{q2} v2 ⊢ ⌜v1 = v2⌝.
   Proof.
-    rewrite 2!high_HighLoc -auth_own_op auth_own_valid.
-    rewrite discrete_valid op_singleton singleton_valid Cinl_op pair_op.
-    by f_equiv=> -[] _ /agree_op_inv/to_agree_inj/leibniz_equiv_iff.
+    rewrite mapsto_eq -own_op -auth_frag_op.
+    rewrite own_valid auth_validI /= discrete_valid.
+    rewrite op_singleton singleton_valid Cinl_op pair_op.
+    by f_equiv=>-[] _ /agree_op_inv/to_agree_inj/leibniz_equiv_iff.
   Qed.
 
   Global Instance heap_ex_mapsto_fractional l : Fractional (λ q, l ↦{q} -)%I.
@@ -588,8 +580,8 @@ Section heap.
 
   Lemma mapsto_valid l q v : l ↦{q} v ⊢ ✓ q.
   Proof.
-    rewrite high_HighLoc auth_own_valid 2!discrete_valid singleton_valid.
-    by apply pure_mono=> -[].
+    rewrite mapsto_eq /mapsto_def own_valid auth_validI /=.
+    rewrite 2!discrete_valid. f_equiv. rewrite singleton_valid. by case.
   Qed.
   Lemma mapsto_valid_2 l q1 q2 v1 v2 : l ↦{q1} v1 ∗ l ↦{q2} v2 ⊢ ✓ (q1 + q2)%Qp.
   Proof.
@@ -597,37 +589,96 @@ Section heap.
     iApply (mapsto_valid l _ v2). by iFrame.
   Qed.
 
+  (** Low locations are disjoint from high locations. *)
+
+  Lemma high_not_low l q v : l ↦{q} v ∗ low l ⊢ False.
+  Proof.
+    rewrite mapsto_eq low_loc lowloc_eq.
+    rewrite -own_op own_valid auth_validI /= discrete_valid.
+    by rewrite op_singleton singleton_valid.
+  Qed.
+
+  (** High locations containing low values can be marked low. *)
+
   Lemma heap_mark_low E l v :
     ↑heapN ⊆ E →
-    heap_ctx -∗ ▷ l ↦ v -∗ ▷ low v ={E}=∗ low l.
+    heap_ctx -∗  l ↦ v -∗ ▷ low v ={E}=∗ low l.
   Proof.
-    rewrite high_eq. iIntros (?) "Hh >(Hl & HL) Hv".
-    iMod (auth_open_strong with "[$Hh $Hl]")
-      as ([h h']) "(%&%&(Hσ&Hlow&Hlive)&Hcl)"; first done.
-    iDestruct (hinv_mark_low with "Hv Hσ Hlow Hlive") as "Hh"=>//.
-    iMod ("Hcl" with "* [Hh]") as "Hl".
-    - iFrame. iPureIntro. exact: to_heap_mark_low.
-    - rewrite low_eq. by iFrame.
+    rewrite mapsto_eq low_loc lowloc_eq. iIntros (?) "Hctx Hl Hv".
+    iInv heapN as (h h' L L') "(>% & Hσ & >Hh & Hlow & Hd)" "Hcl".
+    iDestruct (own_valid_2 with "Hh Hl") as %[??]%auth_valid_discrete_2.
+    case: (to_heap_high_included h h' l 1 v) => // ??.
+    iMod (own_update_2 with "Hh Hl") as "[Hh Hl]".
+    { eapply auth_update. exact: to_heap_mark_low. }
+    iMod ("Hcl" with "[-Hl]"); last by iFrame. iNext.
+    iExists (delete l h), (<[l:=v]> h'), L, L'. iFrame "Hd Hh".
+    rewrite -delete_insert_union //. iFrame "Hσ %".
+    rewrite big_sepM_insert //. by iFrame "Hv Hlow".
+  Qed.
+
+  (** Fresh locations are exclusive. *)
+
+  Global Instance fresh_timeless l : TimelessP (fresh l).
+  Proof. rewrite fresh_eq. apply _. Qed.
+
+  Lemma fresh_exclusive l : fresh l ∗ fresh l ⊢ False.
+  Proof.
+    rewrite fresh_eq -own_op -auth_frag_op.
+    rewrite own_valid auth_validI /= discrete_valid.
+    by rewrite op_singleton singleton_valid.
+  Qed.
+
+  (** Live locations persist and are disjoint from fresh locations. *)
+
+  Global Instance liveloc_timeless l : TimelessP (liveloc l).
+  Proof. rewrite liveloc_eq. apply _. Qed.
+  Global Instance liveloc_persistent l : PersistentP (liveloc l).
+  Proof. rewrite liveloc_eq. apply _. Qed.
+
+  Lemma fresh_not_live l : fresh l ∗ liveloc l -∗ False.
+  Proof.
+    rewrite fresh_eq liveloc_eq -own_op -auth_frag_op.
+    rewrite own_valid auth_validI /= discrete_valid.
+    by rewrite op_singleton singleton_valid.
+  Qed.
+
+  (** Fresh locations can be marked live. *)
+
+  Lemma heap_mark_liveloc E l :
+    ↑heapN ⊆ E →
+    heap_ctx -∗ fresh l ={E}=∗ liveloc l.
+  Proof.
+    rewrite fresh_eq liveloc_eq. iIntros (?) "Hctx Hl".
+    iInv heapN as (h h' L L') "(>% & Hσ & Hh & Hlow & >Hd)" "Hcl".
+    iDestruct (own_valid_2 with "Hd Hl") as %[??]%auth_valid_discrete_2.
+    case: (to_dom_fresh_included L L' l)=>// ??.
+    iMod (own_update_2 with "Hd Hl") as "[Hd Hl]".
+    { eapply auth_update. exact: to_dom_mark_live. }
+    iMod ("Hcl" with "[-Hl]"); last by iFrame. iNext.
+    iExists h, h', (L ∖ {[l]}), ({[l]} ∪ L'). iFrame "Hσ Hh Hlow Hd".
+    by rewrite (dom_mark_live _ _ L L' l).
   Qed.
 
   (** ** Operational rules *)
 
-  Lemma wp_alloc_live p E e v X :
+  Lemma wp_alloc_fresh p E e v :
     to_val e = Some v → ↑heapN ⊆ E →
-    {{{ heap_ctx ∗ live X }}} Alloc e @ p; E
-    {{{ l, RET LocV l; l ↦ v ∗ ⌜l ∉ X⌝ }}}.
+    {{{ heap_ctx }}} Alloc e @ p; E
+    {{{ l, RET LocV l; l ↦ v ∗ fresh l }}}.
   Proof.
-    iIntros (<-%of_to_val ? Φ) "(Hh&#HX) HΦ". rewrite /heap_ctx.
-    iMod (auth_empty (heap_name.1)) as "Ha".
-    iMod (auth_open with "[$Hh $Ha]")
-      as ([h h']) "(%&(Hσ & Hlow & Hlive)&Hcl)"; first done.
-    iApply (wp_alloc_big with "Hσ"); first done. iNext. iIntros (l) "[% Hσ]".
-    iDestruct (live_obs _ l X with "Hlive HX") as "#HXl"; first done.
-    iMod (live_alloc _ l v with "Hlive") as "(Hlive & HL)".
-    iDestruct (hinv_high with "Hσ Hlow Hlive") as "Hh".
-    iMod ("Hcl" with "* [Hh]") as "Hl".
-    - iFrame. iPureIntro. exact: to_heap_alloc_high.
-    - iApply "HΦ". rewrite high_eq. by iFrame.
+    iIntros (<-%of_to_val ? Φ) "Hctx HΦ". rewrite mapsto_eq fresh_eq.
+    iInv heapN as (h h' L L') "(>HD & Hσ & >Hh & Hlow & >Hd)" "Hcl".
+    iApply (wp_alloc_big with "Hσ"); first done. iNext.
+    iIntros (l) "/= [% Hσ]". rewrite insert_union_l.
+    iMod (own_update with "Hh") as "[Hh Hl]".
+    { eapply auth_update_alloc. exact: to_heap_alloc_high. }
+    iDestruct "HD" as %HD.
+    iMod (own_update with "Hd") as "[Hd Hf]".
+    { eapply auth_update_alloc. apply (to_dom_alloc_fresh _ _ l).
+      by rewrite -HD not_elem_of_dom. }
+    iMod ("Hcl" with "[-Hf Hl HΦ]"); last by iApply ("HΦ" with "[$Hl $Hf]").
+    iNext. iExists (<[l:=v]> h), h', ({[l]} ∪ L), L'. iFrame "Hσ Hh Hlow Hd".
+    by rewrite (dom_alloc_fresh _ _ L L').
   Qed.
 
   Lemma wp_load p E l q v :
@@ -635,14 +686,14 @@ Section heap.
     {{{ heap_ctx ∗ ▷ l ↦{q} v }}} Load (Loc l) @ p; E
     {{{ RET v; l ↦{q} v }}}.
   Proof.
-    iIntros (? Φ) "[Hh >Hl] HΦ". rewrite high_eq. iDestruct "Hl" as "[Hl HL]".
-    iMod (auth_open_strong with "[$Hh $Hl]")
-      as ([h h']) "(%&%&(Hσ & Hlow & Hlive)&Hcl)"; first done.
+    iIntros (? Φ) "[Hctx >Hl] HΦ". rewrite mapsto_eq.
+    iInv heapN as (h h' L L') "(>% & Hσ & >Hh & Hlow & Hd)" "Hcl".
+    iDestruct (own_valid_2 with "Hh Hl") as %[??]%auth_valid_discrete_2.
     case: (to_heap_high_included h h' l q v) => // ??.
     iApply (wp_load_big with "Hσ"); [done|exact: lookup_union_Some_l|].
-    iNext. iIntros "Hσ". iDestruct (hinv_intro with "Hσ Hlow Hlive") as "Hh".
-    iMod ("Hcl" with "* [Hh]") as "Hl"; first by eauto.
-    by iApply ("HΦ" with "[$Hl $HL]").
+    iNext. iIntros "Hσ".
+    iMod ("Hcl" with "[-Hl HΦ]"); last by iApply ("HΦ" with "Hl").
+    iNext. iExists h, h', L, L'. by iFrame "Hσ Hh Hlow Hd".
   Qed.
 
   Lemma wp_load_low p E l :
@@ -650,16 +701,15 @@ Section heap.
     {{{ heap_ctx ∗ ▷ low l }}} Load (Loc l) @ p; E
     {{{ v, RET v; low v }}}.
   Proof.
-    iIntros (? Φ) "[Hh >Hl] HΦ". rewrite low_eq. iDestruct "Hl" as "[Hl HL]".
-    iMod (auth_open_strong with "[$Hh $Hl]")
-      as ([h h']) "(%&%&(Hσ & Hlow & Hlive)&Hcl)"; first done.
+    iIntros (? Φ) "[Hctx >Hl] HΦ". rewrite low_loc lowloc_eq.
+    iInv heapN as (h h' L L') "(>% & Hσ & >Hh & Hlow & Hd)" "Hcl".
+    iDestruct (own_valid_2 with "Hh Hl") as %[??]%auth_valid_discrete_2.
     case: (to_heap_low_included h h' l) => // ? [v ?].
     iApply (wp_load_big with "Hσ"); [done|exact: lookup_union_Some_r'|].
     iNext. iIntros "Hσ".
     iDestruct (big_sepM_lookup _ _ l v with "Hlow") as "#Hv"; first done.
-    iDestruct (hinv_intro with "Hσ Hlow Hlive") as "Hh".
-    iMod ("Hcl" with "* [Hh]") as "_"; first by eauto.
-    by iApply ("HΦ" with "Hv").
+    iMod ("Hcl" with "[-HΦ]"); last by iApply ("HΦ" with "Hv").
+    iNext. iExists h, h', L, L'. by iFrame "Hσ Hh Hlow Hd".
   Qed.
 
   Lemma wp_store p E l v' e v :
@@ -667,17 +717,17 @@ Section heap.
     {{{ heap_ctx ∗ ▷ l ↦ v' }}} Store (Loc l) e @ p; E
     {{{ RET UnitV; l ↦ v }}}.
   Proof.
-    iIntros (<-%of_to_val ? Φ) "[Hh >Hl] HΦ".
-    rewrite high_eq. iDestruct "Hl" as "[Hl HL]".
-    iMod (auth_open_strong with "[$Hh $Hl]")
-      as ([h h']) "(%&%&(Hσ & Hlow & Hlive)&Hcl)"; first done.
+    iIntros (<-%of_to_val ? Φ) "[Hctx >Hl] HΦ". rewrite mapsto_eq.
+    iInv heapN as (h h' L L') "(>% & Hσ & >Hh & Hlow & Hd)" "Hcl".
+    iDestruct (own_valid_2 with "Hh Hl") as %[??]%auth_valid_discrete_2.
     case: (to_heap_high_included h h' l 1 v') => // ??.
     iApply (wp_store_big with "Hσ"); [done|exact: lookup_union_Some_l|].
-    iDestruct (live_store_high _ _ l _ v with "Hlive") as "Hlive"=>//.
-    iNext. iIntros "Hσ". iDestruct (hinv_high with "Hσ Hlow Hlive") as "Hh".
-    iMod ("Hcl" with "* [Hh]") as "Hl".
-    - iFrame. iPureIntro. exact: to_heap_store_high.
-    - rewrite high_eq. by iApply ("HΦ" with "[$Hl $HL]").
+    iNext. iIntros "Hσ". iMod (own_update_2 with "Hh Hl") as "[Hh Hl]".
+    { eapply auth_update. exact: to_heap_store_high. }
+    iMod ("Hcl" with "[-Hl HΦ]"); last by iApply ("HΦ" with "Hl").
+    iNext. iExists (<[l:=v]> h), h', L, L'. iFrame "Hh Hlow Hd".
+    rewrite insert_union_l. iFrame "Hσ".
+    by rewrite (dom_store_high _ _ L L' _ v').
   Qed.
 
   Lemma wp_store_low p E l e v :
@@ -685,17 +735,19 @@ Section heap.
     {{{ heap_ctx ∗ ▷ low  l ∗ ▷ low  v }}} Store (Loc l) e @ p; E
     {{{ RET UnitV; True }}}.
   Proof.
-    iIntros (<-%of_to_val ? Φ) "(Hh&>Hl&Hv) HΦ".
-    rewrite low_eq. iDestruct "Hl" as "[Hl HL]".
-    iMod (auth_open_strong with "[$Hh $Hl]")
-      as ([h h']) "(%&%&(Hσ & Hlow & Hlive)&Hcl)"; first done.
+    iIntros (<-%of_to_val ? Φ) "(Hctx & >Hl & Hv) HΦ".
+    rewrite low_loc lowloc_eq.
+    iInv heapN as (h h' L L') "(>% & Hσ & >Hh & Hlow & Hd)" "Hcl".
+    iDestruct (own_valid_2 with "Hh Hl") as %[??]%auth_valid_discrete_2.
     case: (to_heap_low_included h h' l) => // ? [v' ?].
     iApply (wp_store_big with "Hσ"); [done|exact: lookup_union_Some_r'|].
-    iDestruct (live_store_low _ _ _ _ v with "Hlive") as "Hlive"=>//.
-    iNext. iIntros "Hσ".
-    iDestruct (hinv_store_low with "Hv Hσ Hlow Hlive") as "Hh"; try done.
-    iMod ("Hcl" with "* [Hh]") as "_"; last by iApply "HΦ".
-    iFrame. by erewrite to_heap_low_insert_override.
+    iNext. iIntros "Hσ". iMod ("Hcl" with "[-HΦ]"); last by iApply "HΦ".
+    iNext. iExists h, (<[l:=v]>h'), L, L'. iFrame "Hd".
+    rewrite insert_union_r //. iFrame "Hσ".
+    rewrite (to_heap_low_insert_override _ _ l v' v) //. iFrame "Hh".
+    iDestruct (big_sepM_insert_override_2 _ h' l v' v with "Hlow [Hv]")
+      as "Hlow"; auto. iFrame "Hlow".
+    by rewrite (dom_low_insert_override _ _ L L' _ v').
   Qed.
 
   Lemma wp_cas_fail p E l q v' e1 v1 e2 v2 :
@@ -703,16 +755,15 @@ Section heap.
     {{{ heap_ctx ∗ ▷ l ↦{q} v' }}} CAS (Loc l) e1 e2 @ p; E
     {{{ RET LitV (LitBool false); l ↦{q} v' }}}.
   Proof.
-    iIntros (<-%of_to_val <-%of_to_val ?? Φ) "[Hh >Hl] HΦ".
-    rewrite high_eq. iDestruct "Hl" as "[Hl HL]".
-    iMod (auth_open_strong with "[$Hh $Hl]")
-      as ([h h']) "(%&%&(Hσ & Hlow & Hlive)&Hcl)"; first done.
+    iIntros (<-%of_to_val <-%of_to_val ?? Φ) "[Hctx >Hl] HΦ". rewrite mapsto_eq.
+    iInv heapN as (h h' L L') "(>% & Hσ & >Hh & Hlow & Hd)" "Hcl".
+    iDestruct (own_valid_2 with "Hh Hl") as %[??]%auth_valid_discrete_2.
     case: (to_heap_high_included h h' l q v') => // ??.
     iApply (wp_cas_fail_big with "Hσ");
       [done|exact: lookup_union_Some_l|done|].
-    iNext. iIntros "Hσ". iDestruct (hinv_intro with "Hσ Hlow Hlive") as "Hh".
-    iMod ("Hcl" with "* [Hh]") as "Hl".
-    by eauto. by iApply ("HΦ" with "[$Hl $HL]").
+    iNext. iIntros "Hσ".
+    iMod ("Hcl" with "[-Hl HΦ]"); last by iApply ("HΦ" with "Hl").
+    iNext. iExists h, h', L, L'. by iFrame.
   Qed.
 
   Lemma wp_cas_suc p E l e1 v1 e2 v2 :
@@ -720,18 +771,18 @@ Section heap.
     {{{ heap_ctx ∗ ▷ l ↦ v1 }}} CAS (Loc l) e1 e2 @ p; E
     {{{ RET LitV (LitBool true); l ↦ v2 }}}.
   Proof.
-    iIntros (<-%of_to_val <-%of_to_val ? Φ) "[Hh >Hl] HΦ".
-    rewrite high_eq. iDestruct "Hl" as "[Hl HL]".
-    iMod (auth_open_strong with "[$Hh $Hl]")
-      as ([h h']) "(%&%&(Hσ & Hlow & Hlive)&Hcl)"; first done.
+    iIntros (<-%of_to_val <-%of_to_val ? Φ) "[Hcx >Hl] HΦ". rewrite mapsto_eq.
+    iInv heapN as (h h' L L') "(>% & Hσ & >Hh & Hlow & Hd)" "Hcl".
+    iDestruct (own_valid_2 with "Hh Hl") as %[??]%auth_valid_discrete_2.
     case: (to_heap_high_included h h' l 1 v1) => // ??.
-    iDestruct (live_store_high _ _ l _ v2 with "Hlive") as "Hlive"=>//.
     iApply (wp_cas_suc_big with "Hσ");
       [done|exact: lookup_union_Some_l|].
-    iNext. iIntros "Hσ". iDestruct (hinv_high with "Hσ Hlow Hlive") as "Hh".
-    iMod ("Hcl" with "* [Hh]") as "Hl".
-    - iFrame. iPureIntro. exact: to_heap_store_high.
-    - rewrite high_eq. by iApply ("HΦ" with "[$Hl $HL]").
+    iNext. iIntros "Hσ". iMod (own_update_2 with "Hh Hl") as "[Hh Hl]".
+    { eapply auth_update. exact: to_heap_store_high. }
+    iMod ("Hcl" with "[-Hl HΦ]"); last by iApply ("HΦ" with "Hl").
+    iNext. iExists (<[l:=v2]> h), h', L, L'. iFrame "Hh Hlow Hd".
+    rewrite insert_union_l. iFrame "Hσ".
+    by rewrite (dom_store_high _ _ L L' _ v1).
   Qed.
 
   Lemma wp_cas_low p E l e1 v1 e2 v2 :
@@ -739,26 +790,28 @@ Section heap.
     {{{ heap_ctx ∗ ▷ low l ∗ ▷ low v2 }}} CAS (Loc l) e1 e2 @ p; E
     {{{ b, RET LitV (LitBool b); True }}}.
   Proof.
-    iIntros (<-%of_to_val <-%of_to_val ? Φ) "(Hh&>Hl&Hv) HΦ".
-    rewrite low_eq. iDestruct "Hl" as "[Hl HL]".
-    iMod (auth_open_strong with "[$Hh $Hl]")
-      as ([h h']) "(%&%&(Hσ & Hlow & Hlive)&Hcl)"; first done.
+    iIntros (<-%of_to_val <-%of_to_val ? Φ) "(Hctx & >Hl & Hv) HΦ".
+    rewrite low_loc lowloc_eq.
+    iInv heapN as (h h' L L') "(>% & Hσ & >Hh & Hlow & Hd)" "Hcl".
+    iDestruct (own_valid_2 with "Hh Hl") as %[??]%auth_valid_discrete_2.
     case: (to_heap_low_included h h' l) => // ? [v' ?].
     case: (decide (v' = v1)) => [<-|?].
     - iApply (wp_cas_suc_big with "Hσ");
         [done|exact: lookup_union_Some_r'|].
-      iNext. iIntros "Hσ".
-      iDestruct (live_store_low _ _ _ _ v2 with "Hlive") as "Hlive"=>//.
-      iDestruct (hinv_store_low with "Hv Hσ Hlow Hlive") as "Hh"; try done.
-      iMod ("Hcl" with "* [Hh]") as "_"; last by iApply "HΦ".
-      iFrame. by erewrite to_heap_low_insert_override.
+      iNext. iIntros "Hσ". iMod ("Hcl" with "[-HΦ]"); last by iApply "HΦ".
+      iNext. iExists h, (<[l:=v2]>h'), L, L'. iFrame "Hd".
+      rewrite insert_union_r //. iFrame "Hσ".
+      rewrite (to_heap_low_insert_override _ _ l v' v2) //. iFrame "Hh".
+      iDestruct (big_sepM_insert_override_2 _ h' l v' v2 with "Hlow [Hv]")
+        as "Hlow"; auto. iFrame "Hlow".
+      by rewrite (dom_low_insert_override _ _ L L' _ v').
     - iApply (wp_cas_fail_big with "Hσ");
         [done|exact: lookup_union_Some_r'|done|].
-      iNext. iIntros "Hσ". iDestruct (hinv_intro with "Hσ Hlow Hlive") as "Hh".
-      iMod ("Hcl" with "* [Hh]") as "_". by eauto. by iApply "HΦ".
+      iNext. iIntros "Hσ". iMod ("Hcl" with "[-HΦ]"); last by iApply "HΦ".
+      iNext. iExists h, h', L, L'. by iFrame.
   Qed.
 End heap.
-Typeclasses Opaque liveloc' mapsto lowloc' heap_ctx'.
+Typeclasses Opaque mapsto lowloc' fresh' liveloc' heap_ctx'.
 
 (** ** Derived rules *)
 Section derived.
@@ -766,8 +819,33 @@ Section derived.
   Implicit Types e : expr.
   Implicit Types v : val.
 
+  Lemma fresh_not_elem_of_live l L : fresh l -∗ live L -∗ ⌜l ∉ L⌝.
+  Proof.
+    induction L as [|x L Hx IH] using collection_ind_L.
+    { iIntros "Hl _". iPureIntro. exact: not_elem_of_empty. }
+    iIntros "Hl HL".
+    rewrite big_sepS_union; last by move=>?/elem_of_singleton->.
+    rewrite big_sepS_singleton. iDestruct "HL" as "[Hx HL]".
+    iDestruct (IH with "Hl HL") as "%". rewrite not_elem_of_union.
+    case: (decide (l = x))=>?; last first.
+    { iFrame. iPureIntro. by rewrite not_elem_of_singleton. }
+    subst. iExFalso. by iApply (fresh_not_live with "[$Hl $Hx]").
+  Qed.
+
+  Lemma heap_mark_live E l L :
+    ↑heapN ⊆ E →
+    heap_ctx -∗ fresh l -∗ live L ={E}=∗ ⌜l ∉ L⌝ ∗ live ({[l]} ∪ L).
+  Proof.
+    iIntros (?) "Hh Hl HL".
+    iDestruct (fresh_not_elem_of_live with "Hl HL") as "%". iFrame "%".
+    rewrite big_sepS_union //;
+      last by rewrite elem_of_disjoint=>x /elem_of_singleton=>->.
+    rewrite big_sepS_singleton. iFrame "HL".
+    by iApply (heap_mark_liveloc with "Hh Hl").
+  Qed.
+
   (**
-	We can allocate high and low locations, observing
+	We can allocate high and low locations, tracking
 	freshness or not.
   *)
   Lemma wp_alloc p E e v :
@@ -775,21 +853,19 @@ Section derived.
     {{{ heap_ctx }}} Alloc e @ p; E {{{ l, RET LocV l; l ↦ v }}}.
   Proof.
     iIntros (?? Φ) "Hh HΦ".
-    iApply (wp_alloc_live _ _ _ _ ∅ with "[$Hh]"); eauto;
-      first by rewrite /live big_sepS_empty.
-    iNext. iIntros (l) "[Hl _]". by iApply "HΦ".
+    iApply (wp_alloc_fresh with "Hh"); eauto. iNext. iIntros (l) "[Hl _]".
+    by iApply "HΦ".
   Qed.
 
-  Lemma wp_alloc_low_live p E e v X :
+  Lemma wp_alloc_low_fresh p E e v :
     to_val e = Some v → ↑heapN ⊆ E →
-    {{{ heap_ctx ∗ ▷ low v ∗ live X }}} Alloc e @ p; E
-    {{{ l, RET LocV l; low l ∗ ⌜l ∉ X⌝ }}}.
+    {{{ heap_ctx ∗ ▷ low v }}} Alloc e @ p; E
+    {{{ l, RET LocV l; low l ∗ fresh l }}}.
   Proof.
-    iIntros (?? Φ) "(#Hh & Hv & HX) HΦ". rewrite -wp_fupd.
-    iApply (wp_alloc_live with "[$Hh $HX]"); eauto. iNext.
-    iIntros (l) "(Hl & HX)". rewrite [(l ↦ v)%I]later_intro [low _]later_intro.
-    iMod (heap_mark_low with "Hh Hl Hv") as "Hl"; first done.
-    by iApply ("HΦ" with "[$Hl $HX]").
+    iIntros (?? Φ) "[#Hh Hv] HΦ". rewrite -wp_fupd.
+    iApply (wp_alloc_fresh with "Hh"); eauto. iNext. iIntros (l) "[Hl Hf]".
+    rewrite [low _]later_intro. iMod (heap_mark_low with "Hh Hl Hv") as "Hl".
+    done. by iApply ("HΦ" with "[$Hl $Hf]").
   Qed.
 
   Lemma wp_alloc_low p E e v :
@@ -797,10 +873,9 @@ Section derived.
     {{{ heap_ctx ∗ ▷ low v }}} Alloc e @ p; E
     {{{ l, RET LocV l; low l }}}.
   Proof.
-    iIntros (?? Φ) "(Hh & Hv) HΦ".
-    iApply (wp_alloc_low_live _ _ _ _ ∅ with "[$Hh $Hv]"); eauto;
-      first by rewrite /live big_sepS_empty.
-    iNext. iIntros (l) "[Hl _]". by iApply "HΦ".
+    iIntros (?? Φ) "[Hh Hv] HΦ".
+    iApply (wp_alloc_low_fresh with "[$Hh $Hv]"); eauto. iNext.
+    iIntros (l) "[Hl _]". by iApply "HΦ".
   Qed.
 
   (** We can always eliminate low values. *)
